theories/iris_fundamental_br_if.v
@@ -1,0 +1,84 @@
+From mathcomp Require Import ssreflect eqtype seq ssrbool.
+From iris.program_logic Require Import language.
+From iris.proofmode Require Import base tactics classes.
+From iris.base_logic Require Export gen_heap ghost_map proph_map na_invariants.
+From iris.base_logic.lib Require Export fancy_updates.
+From iris.algebra Require Import list.
+From iris.prelude Require Import options.
+
+Require Export iris iris_locations iris_properties iris_atomicity stdpp_aux.
+Require Export iris_rules.
+Require Export datatypes host operations properties opsem typing.
+Require Export iris_logrel iris_fundamental_helpers.
+Require Import iris_fundamental_br.
+Import uPred.
+
+Section fundamental.
+  Import DummyHosts. (* placeholder *)
+
+  Context `{!wfuncG Σ, !wtabG Σ, !wmemG Σ, !wmemsizeG Σ, !wglobG Σ, !wframeG Σ, HWP: host_program_logic, !logrel_na_invs Σ}.
+  
+  (* --------------------------------------------------------------------------------------- *)
+  (* -------------------------------------- EXPRESSIONS ------------------------------------ *)
+  (* --------------------------------------------------------------------------------------- *)
+
+  (* ----------------------------------------- BR_IF --------------------------------------- *)
+  
+  Lemma typing_br_if C i ts : ssrnat.leq (S i) (length (tc_label C)) ->
+                              plop2 C i ts ->
+                              ⊢ semantic_typing (HWP:=HWP) C (to_e_list [BI_br_if i]) (Tf (ts ++ [T_i32]) ts).
+  Proof.
+    iIntros (Hleq Hlookup) "".
+    iIntros (j lh).
+    iIntros "#Hi #Hc" (f vs) "[Hf Hfv] #Hv".
+    unfold interp_expression.
+    
+    iDestruct "Hv" as "[-> | Hv]".
+    { take_drop_app_rewrite_twice 0 1.
+      iApply (wp_wand _ _ _ (λ vs, ⌜vs = trapV⌝ ∗  ↪[frame]f)%I with "[Hf]").
+      { iApply (wp_trap with "[] [Hf]");auto. }
+      iIntros (v0) "[? ?]". iFrame. iExists _. iFrame "∗ #". }
+    iDestruct "Hv" as (ws ->) "Hv".
+    iDestruct (big_sepL2_length with "Hv") as %Hlen.
+    assert (∃ w ws', ws = ws' ++ [w]) as [w [ws' Heq]].
+    { induction ws using rev_ind;eauto. destruct ts =>//. } subst ws.
+    iDestruct (big_sepL2_app_inv with "Hv") as "[Hv' Hw]";[auto|].
+    iSimpl. rewrite fmap_app -app_assoc. iSimpl.
+    iSimpl in "Hw". iDestruct "Hw" as "[Hw _]".
+    iDestruct "Hw" as (z) "->" .
+
+    (* first we reduce the br_if either to nil, or to a br instruction *)
+    iApply wp_wasm_empty_ctx.
+    iApply iRewrite_nil_r_ctx. rewrite -app_assoc.
+    iApply wp_base_push;[apply v_to_e_is_const_list|].
+    iApply iRewrite_nil_r_ctx.
+    iApply (wp_seq_ctx _ _ _ (λne (vs : leibnizO val), ⌜vs = immV [] ∨ vs = brV i [] []⌝ ∗ ↪[frame] f)%I).
+    iSplitR;[iIntros "[[%Hcontr|%Hcontr] _]"; done|].
+    iSplitL "Hf".
+    { destruct (Wasm_int.Int32.eq_eqP z (Wasm_int.int_zero i32m)).
+      { iApply (wp_br_if_false with "Hf");auto. }
+      { iApply (wp_br_if_true with "Hf");auto. iNext. iIntros "Hf".
+        iApply wp_value.
+        { instantiate (1:=brV i [] []). done. }
+        iFrame. iRight. auto. }
+    }
+
+    iIntros (w) "[[-> | ->] Hf]".
+    { (* if the br does not happen, we return and get the result of type ts *)
+      iSimpl. iIntros (LI Hfill%lfilled_Ind_Equivalent);inversion Hfill;simplify_eq.
+      repeat erewrite app_nil_r.
+      iApply wp_value.
+      { instantiate (1:=immV ws'). done. }
+      iSplitR;[|iExists _;iFrame].
+      iLeft. iRight. iExists _. iSplit;eauto. }
+
+    (* otherwise, we continue as reason about the br as in typing_br *)
+    iDestruct (typing_br _ _ [] _ ts with "Hi Hc [$] []") as "Hbr";[eauto..|].
+    { rewrite app_nil_l. iRight. iExists _;eauto. }
+    unfold interp_expression.
+    iIntros (LI Hfill%lfilled_Ind_Equivalent);inversion Hfill;simplify_eq.
+    repeat erewrite app_nil_r.
+    iApply "Hbr".
+  Qed.
+
+End fundamental.
