theories/iris_fundamental_cvtop.v
@@ -1,0 +1,109 @@
+From mathcomp Require Import ssreflect eqtype seq ssrbool.
+From iris.program_logic Require Import language.
+From iris.proofmode Require Import base tactics classes.
+From iris.base_logic Require Export gen_heap ghost_map proph_map na_invariants.
+From iris.base_logic.lib Require Export fancy_updates.
+From iris.algebra Require Import list.
+From iris.prelude Require Import options.
+
+Require Export iris iris_locations iris_properties iris_atomicity stdpp_aux.
+Require Export iris_rules.
+Require Export datatypes host operations properties opsem typing.
+Require Export iris_logrel iris_fundamental_helpers.
+Import uPred.
+
+Section fundamental.
+  Import DummyHosts. (* placeholder *)
+
+  Context `{!wfuncG Σ, !wtabG Σ, !wmemG Σ, !wmemsizeG Σ, !wglobG Σ, !wframeG Σ, HWP: host_program_logic, !logrel_na_invs Σ}.
+  
+  (* --------------------------------------------------------------------------------------- *)
+  (* -------------------------------------- EXPRESSIONS ------------------------------------ *)
+  (* --------------------------------------------------------------------------------------- *)
+
+  Lemma interp_value_cvt t1 sx w1 v :
+    cvt t1 sx w1 = Some v ->
+    ⊢ interp_value (Σ:=Σ) t1 v.
+  Proof.
+    iIntros (Hcvt).
+    unfold interp_value.
+    unfold cvt in Hcvt.
+    destruct t1,v;eauto.
+    all: unfold option_map in Hcvt.
+    all: (destruct (cvt_i32 sx w1);done) +
+           (destruct (cvt_i64 sx w1);done) +
+           (destruct (cvt_f32 sx w1);done) +
+           (destruct (cvt_f64 sx w1);done) + auto.
+  Qed.
+
+  Lemma interp_value_reinterpret t1 w1 :
+    ⊢ interp_value (Σ:=Σ) t1 (wasm_deserialise (bits w1) t1).
+  Proof.
+    destruct t1;simpl;eauto.
+  Qed.
+    
+  (* ----------------------------------------- CVTOP --------------------------------------- *)
+
+  Lemma typing_cvtop_convert C t1 t2 sx : ⊢ semantic_typing (HWP:=HWP) C (to_e_list [BI_cvtop t1 CVO_convert t2 sx]) (Tf [t2] [t1]).
+  Proof.
+    unfold semantic_typing, interp_expression.
+    iIntros (i lh).
+    iIntros "#Hi [%Hlh_base [%Hlh_len [%Hlh_valid #Hcont]]]" (f vs) "[Hf Hfv] #Hv".
+    iDestruct "Hv" as "[-> | Hv]".
+    { take_drop_app_rewrite_twice 0 1.
+      iApply (wp_wand _ _ _ (λ vs, ⌜vs = trapV⌝ ∗  ↪[frame]f)%I with "[Hf]").
+      { iApply (wp_trap with "[] [$]");auto. }
+      iIntros (v0) "[? ?]". iFrame. iExists _. iFrame "∗ #". }
+    iDestruct "Hv" as (ws ->) "Hv".
+    iDestruct (big_sepL2_length with "Hv") as %Hlen.
+    destruct ws as [|w1 ws];[done|destruct ws;[|done]].
+    iSimpl in "Hv".
+    iDestruct "Hv" as "[Hv1 _]".
+    iSimpl.
+    
+    iApply (wp_wand _ _ _ (λne vs, interp_val [t1] vs ∗ ↪[frame] f)%I with "[Hf]").
+    { iAssert (⌜types_agree t2 w1⌝)%I as %Htyp.
+      { destruct t2. all:iDestruct "Hv1" as (?) "->";eauto. }
+      destruct (cvt t1 sx w1) eqn:Hsome.      
+      { iApply (wp_cvtop_convert with "Hf");eauto.
+        iSimpl. iRight. iExists _. iSplit;eauto.
+        iSimpl. iSplit;[|done]. iApply interp_value_cvt. eauto. }
+      { iApply (wp_cvtop_convert_failure with "Hf");eauto.
+        iSimpl. by iLeft. }
+    }
+
+    iIntros (v) "[H Hf]".
+    iFrame. iExists _. iFrame.
+  Qed.
+
+  Lemma typing_cvtop_reinterpret C t1 t2 : ⊢ semantic_typing (HWP:=HWP) C (to_e_list [BI_cvtop t1 CVO_reinterpret t2 None]) (Tf [t2] [t1]).
+  Proof.
+    unfold semantic_typing, interp_expression.
+    iIntros (i lh).
+    iIntros "#Hi [%Hlh_base [%Hlh_len [%Hlh_valid #Hcont]]]" (f vs) "[Hf Hfv] #Hv".
+    iDestruct "Hv" as "[-> | Hv]".
+    { take_drop_app_rewrite_twice 0 1.
+      iApply (wp_wand _ _ _ (λ vs, ⌜vs = trapV⌝ ∗  ↪[frame]f)%I with "[Hf]").
+      { iApply (wp_trap with "[] [$]");auto. }
+      iIntros (v0) "[? ?]". iFrame. iExists _. iFrame "∗ #". }
+    iDestruct "Hv" as (ws ->) "Hv".
+    iDestruct (big_sepL2_length with "Hv") as %Hlen.
+    destruct ws as [|w1 ws];[done|destruct ws;[|done]].
+    iSimpl in "Hv".
+    iDestruct "Hv" as "[Hv1 _]".
+    iSimpl.
+    
+    iApply (wp_wand _ _ _ (λne vs, interp_val [t1] vs ∗ ↪[frame] f)%I with "[Hf]").
+    { iAssert (⌜types_agree t2 w1⌝)%I as %Htyp.
+      { destruct t2. all:iDestruct "Hv1" as (?) "->";eauto. }
+      iApply (wp_cvtop_reinterpret with "Hf");eauto.
+      iSimpl. iRight. iExists _. iSplit;eauto.
+      iSimpl. iSplit;[|done]. iApply interp_value_reinterpret.
+    }
+
+    iIntros (v) "[H Hf]".
+    iFrame. iExists _. iFrame.
+  Qed.
+
+
+End fundamental.
