theories/iris_fundamental_unop.v
@@ -39,7 +39,7 @@ Section fundamental.
     unfold semantic_typing, interp_expression.
     iIntros (Hunop i lh).
     iIntros "#Hi [%Hlh_base [%Hlh_len [%Hlh_valid #Hcont]]]".
-    iIntros (f vs) "[Hf #Hfv] #Hv".
+    iIntros (f vs) "[Hf Hfv] #Hv".
     iDestruct "Hv" as "[-> | Hv]".
     { take_drop_app_rewrite_twice 0 1.
       iApply (wp_wand _ _ _ (λ vs, ⌜vs = trapV⌝ ∗  ↪[frame]f)%I with "[Hf]").
@@ -54,7 +54,7 @@ Section fundamental.
       iApply (wp_wand _ _ _ (λ v, ⌜v = immV [app_unop op w]⌝ ∗ ↪[frame] f)%I with "[Hf]").
       { iApply (wp_unop with "Hf");eauto. }
       iIntros (w0) "[-> Hf]".
-      iSplitR;[|eauto].
+      iSplitR;[|iExists _;iFrame].
       iLeft. iRight.
       iExists [app_unop op w]. iSplit;auto.
       iSimpl. iSplit;auto.
