theories/iris_rules_structural_with_trap.v
@@ -517,8 +517,6 @@ Proof.
   } } }
 Qed.
 
-
-
 Lemma wp_val_return' (s : stuckness) (E : coPset) (Φ : val -> iProp Σ) vs vs' es' es'' n f0 Φf :
   const_list vs ->
   ↪[frame] f0 -∗
